rocq-skylabs-brick/tests/float_support.v
@@ -1,0 +1,232 @@
+(*
+ * Copyright (c) 2026 SkyLabs AI, Inc.
+ * This software is distributed under the terms of the BedRock Open-Source License.
+ * See the LICENSE-BedRock file in the repository root for details.
+ *)
+Require Import Stdlib.ZArith.BinInt.
+Require Import Stdlib.micromega.Lia.
+Require Import skylabs.lang.cpp.syntax.
+Require Import skylabs.lang.cpp.syntax.supported.
+Require Import skylabs.lang.cpp.semantics.genv.
+Require Import skylabs.lang.cpp.semantics.values.
+Require Import skylabs.lang.cpp.semantics.cast.
+Require Import skylabs.lang.cpp.semantics.cast_operator.
+
+Open Scope pstring_scope.
+Open Scope Z_scope.
+
+Definition one_float : Expr :=
+  Efloat Ffloat (fp_of_bits Ffloat 1065353216%Z) Tfloat.
+
+Definition one_double : Expr :=
+  Efloat Fdouble (fp_of_bits Fdouble 4607182418800017408%Z) Tdouble.
+
+Example support_accepts_float_type : check.type Tfloat = check.OK.
+Proof. reflexivity. Qed.
+
+Example support_accepts_double_type : check.type Tdouble = check.OK.
+Proof. reflexivity. Qed.
+
+Example support_rejects_float16_type : check.type Tfloat16 <> check.OK.
+Proof. vm_compute. discriminate. Qed.
+
+Example support_rejects_longdouble_type : check.type Tlongdouble <> check.OK.
+Proof. vm_compute. discriminate. Qed.
+
+Example support_rejects_float128_type : check.type Tfloat128 <> check.OK.
+Proof. vm_compute. discriminate. Qed.
+
+Example support_accepts_supported_float_literal : check.expr one_float = check.OK.
+Proof. reflexivity. Qed.
+
+Example support_rejects_unsupported_float_literal :
+  check.expr (Efloat Ffloat16 tt Tfloat16) <> check.OK.
+Proof. vm_compute. discriminate. Qed.
+
+Example support_accepts_float_to_double_cast :
+  check.expr (Ecast (Cfloat Tdouble) (Evar "f" Tfloat)) = check.OK.
+Proof. reflexivity. Qed.
+
+Example support_rejects_longdouble_to_double_cast :
+  check.expr (Ecast (Cfloat Tdouble) (Evar "ld" Tlongdouble)) <> check.OK.
+Proof. vm_compute. discriminate. Qed.
+
+Example support_rejects_int_to_float16_cast :
+  check.expr (Ecast (Cint2float Tfloat16) (Eint 0 Tint)) <> check.OK.
+Proof. vm_compute. discriminate. Qed.
+
+Example support_rejects_float128_to_int_cast :
+  check.expr (Ecast (Cfloat2int Tint) (Evar "q" Tfloat128)) <> check.OK.
+Proof. vm_compute. discriminate. Qed.
+
+Example support_accepts_float_add :
+  check.expr (Ebinop Badd one_float one_float Tfloat) = check.OK.
+Proof. reflexivity. Qed.
+
+Example support_rejects_float_mod :
+  check.expr (Ebinop Bmod one_float one_float Tfloat) <> check.OK.
+Proof. vm_compute. discriminate. Qed.
+
+Example support_rejects_float_bitwise :
+  check.expr (Ebinop Band one_float one_float Tfloat) <> check.OK.
+Proof. vm_compute. discriminate. Qed.
+
+Example support_rejects_float_shift :
+  check.expr (Ebinop Bshl one_float (Eint 1 Tint) Tfloat) <> check.OK.
+Proof. vm_compute. discriminate. Qed.
+
+Example support_rejects_pointer_plus_float :
+  check.expr (Ebinop Badd (Evar "p" (Tptr Tint)) one_float (Tptr Tint)) <> check.OK.
+Proof. vm_compute. discriminate. Qed.
+
+Example support_rejects_float_increment :
+  check.expr (Epreinc (Evar "f" Tfloat) Tfloat) <> check.OK.
+Proof. vm_compute. discriminate. Qed.
+
+Example usual_float_arith_rejects_longdouble tu :
+  usual_float_arith tu Tlongdouble Tdouble = None.
+Proof. reflexivity. Qed.
+
+Example convert_type_rejects_pointer_plus_float tu :
+  convert_type_op tu Badd (Tptr Tint) Tfloat = None.
+Proof. reflexivity. Qed.
+
+Example convert_type_rejects_float_mod tu :
+  convert_type_op tu Bmod Tfloat Tfloat = None.
+Proof. reflexivity. Qed.
+
+Example convert_type_accepts_float_double_add tu :
+  convert_type_op tu Badd Tfloat Tdouble = Some (Tdouble, Tdouble, Tdouble).
+Proof. reflexivity. Qed.
+
+Example convert_rejects_unsupported_float_to_int {σ : genv} tu v v' :
+  @convert σ tu Tlongdouble Tint v v' = False.
+Proof. reflexivity. Qed.
+
+Definition f32_one : fp_carrier Ffloat := fp_of_bits Ffloat 1065353216%Z.
+Definition f64_one : fp_carrier Fdouble := fp_of_bits Fdouble 4607182418800017408%Z.
+Definition f32_neg_zero : fp_carrier Ffloat := fp_of_bits Ffloat 2147483648%Z.
+Definition f64_neg_zero : fp_carrier Fdouble := fp_of_bits Fdouble 9223372036854775808%Z.
+Definition f32_inf : fp_carrier Ffloat := fp_of_bits Ffloat 2139095040%Z.
+Definition f64_inf : fp_carrier Fdouble := fp_of_bits Fdouble 9218868437227405312%Z.
+Definition f32_nan : fp_carrier Ffloat := fp_default_nan Ffloat.
+Definition f64_nan : fp_carrier Fdouble := fp_default_nan Fdouble.
+
+Example has_type_prop_float_value {σ : genv} :
+  has_type_prop (Vfloat_ Ffloat f32_one) Tfloat.
+Proof. apply has_float_type. reflexivity. Qed.
+
+Example has_type_prop_double_value {σ : genv} :
+  has_type_prop (Vfloat_ Fdouble f64_one) Tdouble.
+Proof. apply has_float_type. reflexivity. Qed.
+
+Example has_type_prop_rejects_mismatched_float_index {σ : genv} :
+  ~ has_type_prop (Vfloat_ Ffloat f32_one) Tdouble.
+Proof.
+  intros Hty.
+  apply (has_type_prop_float_inv Fdouble) in Hty; last reflexivity.
+  destruct Hty as [f Hf]. discriminate Hf.
+Qed.
+
+Example fp32_to_of_bits_roundtrip bits :
+  (0 <= bits < 2 ^ 32)%Z -> fp_to_bits Ffloat (fp_of_bits Ffloat bits) = bits.
+Proof. intros Hbits. apply fp_to_of_bits; [reflexivity|exact Hbits]. Qed.
+
+Example fp64_to_of_bits_roundtrip bits :
+  (0 <= bits < 2 ^ 64)%Z -> fp_to_bits Fdouble (fp_of_bits Fdouble bits) = bits.
+Proof. intros Hbits. apply fp_to_of_bits; [reflexivity|exact Hbits]. Qed.
+
+Example fp32_of_to_bits_roundtrip f : fp_of_bits Ffloat (fp_to_bits Ffloat f) = f.
+Proof. apply fp_of_to_bits. Qed.
+
+Example fp64_of_to_bits_roundtrip f : fp_of_bits Fdouble (fp_to_bits Fdouble f) = f.
+Proof. apply fp_of_to_bits. Qed.
+
+Example default_float_zero : get_default Tfloat = Some (Vfloat_ Ffloat (fp_zero Ffloat)).
+Proof. reflexivity. Qed.
+
+Example default_double_zero : get_default Tdouble = Some (Vfloat_ Fdouble (fp_zero Fdouble)).
+Proof. reflexivity. Qed.
+
+Example default_longdouble_unsupported : get_default Tlongdouble = None.
+Proof. reflexivity. Qed.
+
+Example float_bool_plus_zero_false : is_true (Vfloat_ Ffloat (fp_zero Ffloat)) = Some false.
+Proof. simpl. rewrite fp_is_true_zero_Ffloat. reflexivity. Qed.
+
+Example double_bool_plus_zero_false : is_true (Vfloat_ Fdouble (fp_zero Fdouble)) = Some false.
+Proof. simpl. rewrite fp_is_true_zero_Fdouble. reflexivity. Qed.
+
+Example float_bool_minus_zero_false : is_true (Vfloat_ Ffloat f32_neg_zero) = Some false.
+Proof. vm_compute. reflexivity. Qed.
+
+Example double_bool_minus_zero_false : is_true (Vfloat_ Fdouble f64_neg_zero) = Some false.
+Proof. vm_compute. reflexivity. Qed.
+
+Example float_bool_nonzero_true : is_true (Vfloat_ Ffloat f32_one) = Some true.
+Proof. vm_compute. reflexivity. Qed.
+
+Example double_bool_nonzero_true : is_true (Vfloat_ Fdouble f64_one) = Some true.
+Proof. vm_compute. reflexivity. Qed.
+
+Example float_bool_inf_true : is_true (Vfloat_ Ffloat f32_inf) = Some true.
+Proof. vm_compute. reflexivity. Qed.
+
+Example double_bool_inf_true : is_true (Vfloat_ Fdouble f64_inf) = Some true.
+Proof. vm_compute. reflexivity. Qed.
+
+Example float_bool_nan_true : is_true (Vfloat_ Ffloat f32_nan) = Some true.
+Proof. vm_compute. reflexivity. Qed.
+
+Example double_bool_nan_true : is_true (Vfloat_ Fdouble f64_nan) = Some true.
+Proof. vm_compute. reflexivity. Qed.
+
+Example float_nan_compare_unordered : fp_compare Ffloat f32_nan f32_nan = None.
+Proof. vm_compute. reflexivity. Qed.
+
+Example double_nan_compare_unordered : fp_compare Fdouble f64_nan f64_nan = None.
+Proof. vm_compute. reflexivity. Qed.
+
+Example float_nan_eq_false :
+  (if fp_compare Ffloat f32_nan f32_nan is Some Eq then true else false) = false.
+Proof. vm_compute. reflexivity. Qed.
+
+Example float_nan_neq_true :
+  (if fp_compare Ffloat f32_nan f32_nan is Some Eq then false else true) = true.
+Proof. vm_compute. reflexivity. Qed.
+
+Example float_nan_ordered_lt_false :
+  (if fp_compare Ffloat f32_nan f32_nan is Some Lt then true else false) = false.
+Proof. vm_compute. reflexivity. Qed.
+
+Example conv_float_identity_example {σ : genv} tu :
+  conv_float tu Tfloat Tfloat (Vfloat_ Ffloat f32_one) (Vfloat_ Ffloat f32_one).
+Proof. apply conv_float_id. reflexivity. Qed.
+
+Example conv_float_to_bool_example {σ : genv} tu :
+  conv_float tu Tfloat Tbool (Vfloat_ Ffloat f32_one) (Vbool true).
+Proof. change true with (fp_is_true Ffloat f32_one). apply conv_float_to_bool. reflexivity. Qed.
+
+Example conv_float_widen_example {σ : genv} tu :
+  conv_float tu Tfloat Tdouble (Vfloat_ Ffloat f32_one)
+    (Vfloat_ Fdouble (fp_float_to_double f32_one)).
+Proof. apply conv_float_widen. Qed.
+
+Example conv_float_narrow_example {σ : genv} tu :
+  conv_float tu Tdouble Tfloat (Vfloat_ Fdouble f64_one)
+    (Vfloat_ Ffloat (fp_double_to_float f64_one)).
+Proof. apply conv_float_narrow. Qed.
+
+Example conv_float_int_to_float_example {σ : genv} tu :
+  conv_float tu Tint Tfloat (Vint 1) (Vfloat_ Ffloat (fp_of_Z Ffloat 1)).
+Proof.
+  eapply ConvFloatIntToFloat; [reflexivity|reflexivity|].
+  rewrite -has_int_type /bitsize.bound /bitsize.min_val /bitsize.max_val /=; lia.
+Qed.
+
+Example conv_float_float_to_int_example {σ : genv} tu :
+  conv_float tu Tfloat Tint (Vfloat_ Ffloat f32_one) (Vint 1).
+Proof.
+  eapply ConvFloatToInt; [reflexivity|reflexivity|vm_compute; reflexivity|].
+  rewrite -has_int_type /bitsize.bound /bitsize.min_val /bitsize.max_val /=; lia.
+Qed.
